update Unification.lean

Plfl/ClosConv.lean
@@ -8,32 +8,35 @@ inductive Val : Type
   | tuple : List Val → Val
 
 inductive Exp : Type
-  -- | letVal : String → Val → Exp → Exp
   | letProj {n : Nat} : String → Fin n → Val → Exp → Exp
   | app : Val → List Val → Exp
   | halt : Val → Exp
 end
 
+@[simp]
+def Exp.letVal (x : String) (v : Val) (e : Exp) : Exp :=
+  .app (.lam [x] e) [v]
+
+@[simp]
+def Exp.letVals (xvs : List (String × Val)) : Exp →  Exp :=
+  xvs.foldr (fun ⟨x, v⟩ => Exp.letVal x v)
+
 mutual
+@[simp]
 def Val.subst (x : String) (s : Val) : Val → Val
+  | .num n => .num n
   | .var y => if x = y then s else Val.var y
   | .lam ys e => .lam ys (if ys.elem x then e else Exp.subst x s e)
-  | v => v
+  | .tuple vs => .tuple (List.map (fun ⟨a, _⟩ => Val.subst x s a) vs.attach)
 
-def Val.substs (x : String) (s : Val) (vs : List Val) : List Val :=
-  vs.map (Val.subst x s)
-
+@[simp]
 def Exp.subst (x : String) (s : Val) : Exp → Exp
-  -- | .letVal y v e => .letVal y (Val.subst x s v) (Exp.subst x s e)
   | .letProj y i v t => .letProj y i (Val.subst x s v) (Exp.subst x s t)
-  | .app v us => .app (Val.subst x s v) (Val.substs x s us)
+  | .app v us => .app (Val.subst x s v) (List.map (fun ⟨a, _⟩ => Val.subst x s a) us.attach)
   | .halt v => .halt (Val.subst x s v)
 end
-termination_by
-  Val.subst _ _ v => sizeOf v
-  Val.substs _ _ vs => Nat.sum (List.map sizeOf vs)
-  Exp.subst _ _ e => sizeOf e
 
+notation:90 "[" x "↦" s "]" v:80 => Val.subst x s v
 notation:90 "[" x "↦" s "]" e:80 => Exp.subst x s e
 
 def Exp.msubst (subs : List (String × Val)) : Exp → Exp
@@ -41,5 +44,254 @@ def Exp.msubst (subs : List (String × Val)) : Exp → Exp
 
 inductive Step : Exp → Exp → Prop
   | app_abs {xs e vs} : Step (.app (.lam xs e) vs) (e.msubst (List.zip xs vs))
-  | halt {v} : Step (.halt v) (.halt v)
   | letProj_tuple {x vs e} {i : Fin vs.length} : Step (.letProj x i (Val.tuple vs) e) ([x ↦ vs.get i] e)
+
+infix:40 " ——→ " => Step
+
+inductive Steps : Exp → Exp → Prop
+  | halt {e v}      : e = .halt v → Steps e e
+  | step {e e' e''} : e ——→ e' → Steps e' e'' → Steps e e''
+
+infix:40 " ——→* " => Steps
+
+theorem steps_composite {e e' e''} : e ——→* e' → e' ——→* e'' → e ——→* e'' := by
+  intro h1
+  intro h2
+  induction h1
+  case halt _ => exact h2
+  case step e1 e1' e1'' h3 _ h5 =>
+    have h6 := h5 h2
+    exact Steps.step h3 h6
+
+@[simp]
+def halts (e : Exp) (v : Val) : Prop := e ——→* .halt v
+
+infix:50 " ⇓ " => halts
+
+infix:50 " ≈ " => Eq
+
+mutual
+def Val.freeVars : Val → List String
+  | .num _ => []
+  | .var x => [x]
+  | .lam xs e => e.freeVars.removeAll xs
+  | .tuple vs => vs.attach.foldl (fun acc ⟨v, _⟩ => (acc ++ v.freeVars).eraseDups) []
+termination_by v => sizeOf v
+
+def Exp.freeVars : Exp → List String
+  | .letProj x _ v e => (v.freeVars ++ e.freeVars.erase x).eraseDups
+  | .app v vs => (vs.attach.foldl (fun acc ⟨v, _⟩ => (acc ++ v.freeVars).eraseDups) (v.freeVars))
+  | .halt v => v.freeVars
+termination_by e => sizeOf e
+end
+
+theorem enumFrom_dec {i j : Nat} {x : α} {xs : List α} : ⟨j, x⟩ ∈ xs.enumFrom i → j < i + xs.length := by
+  intro h
+  cases xs
+  case nil => simp at h
+  case cons hd tl =>
+    simp at h
+    cases h with
+    | inl h => simp [h]
+    | inr h =>
+        rw [List.length_cons, Nat.add_left_comm, Nat.add_comm]
+        apply enumFrom_dec h
+termination_by xs.length
+
+mutual
+def Val.clos_conv : Val → Val
+  | .num n => .num n
+  | .var x => .var x
+  | .lam xs e =>
+      let c := "c"
+      let ys := Val.freeVars (.lam xs e)
+      let enum_ys := ys.enumFrom 1
+      let exp := enum_ys.attach.foldr (fun ⟨⟨i, y⟩, p⟩ => .letProj y (.mk i (enumFrom_dec p)) (.var c)) e.clos_conv
+      .tuple (.lam (c :: xs) exp :: (ys.map Val.var))
+  | .tuple vs => .tuple (List.map (fun ⟨a, _⟩ => Val.clos_conv a) vs.attach)
+termination_by v => sizeOf v
+
+def Exp.clos_conv : Exp → Exp
+  | .letProj x i v e => .letProj x i (Val.clos_conv v) (Exp.clos_conv e)
+  | .app v vs =>
+      let c := "c"
+      let f := "f"
+      let prf := Nat.zero_lt_succ (vs.length)
+      .letVal c v.clos_conv <|
+      .letProj f (.mk 0 prf) (Val.var c) <|
+      .app (Val.var c) (List.map (fun ⟨a, _⟩ => Val.clos_conv a) vs.attach)
+  | .halt v => .halt (Val.clos_conv v)
+termination_by e => sizeOf e
+end
+
+notation:80 "⟦" v "⟧" => Val.clos_conv v
+notation:80 "⟦" e "⟧" => Exp.clos_conv e
+
+def Val.rel (v v' : Val) : Prop := Val.clos_conv v = v'
+def Exp.rel (e e' : Exp) : Prop := Exp.clos_conv e = e'
+
+infix:50 " ≳ " => Val.rel
+infix:50 " ≳ " => Exp.rel
+
+theorem clos_conv_satisfies_rel {e : Exp} : e ≳ ⟦ e ⟧ := by
+  simp [Exp.rel, Exp.clos_conv]
+
+theorem rel_implies_equal {e e' : Exp} : e ≳ e' → ⟦ e ⟧ ≈ e' := by
+  intro h
+  simp [Exp.rel] at h
+  rw [h]
+
+theorem Val.subst_preserves {v : Val} {v' : Val} : [x ↦ v] v' ≳ [x ↦ ⟦v⟧] ⟦v'⟧ := by
+  cases v'
+  case num n => simp [Val.clos_conv, Val.rel]
+  case var y =>
+    simp [Val.clos_conv, Val.rel]
+    split
+    . trivial
+    . simp [Val.clos_conv]
+  case lam ys e =>
+    simp [Val.clos_conv]
+    split
+    case isTrue h =>
+      simp [Val.rel, Val.clos_conv]
+      apply And.intro
+      . split
+        case isTrue => trivial
+        case isFalse h1 =>
+          simp at h1
+          have h2 := h1.right
+          contradiction
+      . simp [Function.comp_def, List.attach_map_val]
+        intro a
+        intro h1
+        split
+        case isTrue h2 =>
+          rw [← h2] at h1
+          sorry
+        trivial
+    case isFalse h =>
+      simp [Val.rel, Val.clos_conv]
+      apply And.intro
+      .
+        sorry
+      . sorry
+  case tuple vs => sorry -- simp [Val.clos_conv, Val.rel]
+
+theorem Exp.subst_preserves {e : Exp} {v : Val} : [x ↦ v] e ≳ [x ↦ ⟦v⟧] ⟦e⟧ := by
+  cases e
+  case halt v' =>
+    simp [Exp.clos_conv, Exp.rel]
+    exact Val.subst_preserves
+  case letProj n x' i v' e' =>
+    simp
+    simp [Exp.clos_conv, Exp.rel]
+    apply And.intro Val.subst_preserves Exp.subst_preserves
+  case app v' us =>
+    simp
+    simp [Exp.clos_conv, Exp.rel]
+    apply And.intro
+    . sorry
+    . exact Val.subst_preserves
+
+theorem simulation {e₁ e₁' e₂ : Exp} : e₁ ≳ e₁' ∧ e₁ ——→ e₂ → ∃ e₂', e₂ ≳ e₂' ∧ e₁' ——→* e₂' := by
+  intro h1
+  cases h1.right
+  case app_abs xs e vs =>
+    have h2 := h1.left
+    simp [Exp.rel, Exp.clos_conv, Val.clos_conv] at h2
+    apply Exists.intro (⟦e.msubst (xs.zip vs)⟧)
+    apply And.intro
+    . simp [Exp.rel]
+    . rw [← h2]
+      apply Steps.step .app_abs
+      . simp [Exp.msubst]
+        apply Steps.step
+        . -- apply Step.letProj_tuple (x := "f") (i := ⟨0, _⟩)
+          sorry
+        . sorry
+        sorry
+  case letProj_tuple x vs e i =>
+    have h2 := h1.left
+    simp [Exp.rel, Exp.clos_conv, Val.clos_conv] at h2
+    apply Exists.intro (⟦e.subst x (vs.get i)⟧)
+    apply And.intro
+    . simp [Exp.rel]
+    . rw [← h2]
+      apply Steps.step
+      . simp [List.attach_map_val]
+        have h3 : Fin vs.length = Fin (List.map Val.clos_conv vs).length := by
+          rw [List.length_map]
+        apply Step.letProj_tuple (x := x) (i := i) (vs := List.map Val.clos_conv vs)
+        sorry
+      . sorry
+      . trivial
+
+theorem simulation_terminate {e e' : Exp} {v: Val} : e ≳ e' ∧ e ⇓ v → ∃ v', e' ⇓ v' ∧ ⟦ v ⟧ ≈ v' := by
+  intro h1
+  have h2 := h1.left
+  have h3 := h1.right
+  simp at h3
+  cases h3
+  case halt =>
+    apply Exists.intro (⟦ v ⟧)
+    cases h2
+    simp [Exp.clos_conv]
+    apply Steps.halt (v := ⟦ v ⟧)
+    trivial
+  case step e1 h4 h5 =>
+    have ⟨e1', h6⟩ := simulation (And.intro h2 h4)
+    have h7 := h6.left
+    rw [← halts] at h5
+    have ⟨v', h8⟩ := simulation_terminate (And.intro h7 h5)
+    apply Exists.intro v'
+    apply And.intro
+    have h9 := h8.left
+    simp at h9
+    exact steps_composite h6.right h9
+    exact h8.right
+termination_by h => sizeOf h.right
+
+theorem completeness {e v} : e ⇓ v → ∃ v', ⟦ e ⟧ ⇓ v' ∧ ⟦ v ⟧ ≈ v' := by
+  intro h1
+  have h2 := simulation_terminate (e := e) (v := v) (e' := ⟦ e ⟧)
+  have h3 := And.intro (clos_conv_satisfies_rel (e := e)) h1
+  exact h2 h3
+
+/-
+theorem soundness {e v'} : ⟦ e ⟧ ⇓ v' → ∃ v, e ⇓ v ∧ ⟦ v ⟧ ≈ v' := by
+  intro h1
+  cases e
+  case halt v =>
+    apply Exists.intro v
+    simp [Exp.clos_conv] at h1
+    apply And.intro
+    exact Steps.halt rfl
+    cases h1
+    trivial
+    trivial
+  case letProj n x i v e =>
+    cases v
+    case tuple vs =>
+      simp [Exp.clos_conv] at h1
+      cases h1
+      case step e' h2 h3 =>
+        simp [Val.clos_conv] at h2
+        cases h2
+        case letProj_tuple i =>
+          simp at h3
+          rw [← Exp.subst_preserves] at h3
+          have ⟨v, h4⟩ := soundness h3
+          apply Exists.intro v
+          apply And.intro
+          simp
+          apply Steps.step (e' := [x ↦ vs.attach[↑i].val] e)
+          sorry
+          exact h4.left
+          exact h4.right
+    case lam ys e' =>
+      simp [Exp.clos_conv] at h1
+      cases h1
+      sorry
+    case num _ => sorry
+    case var _ => sorry
+  case app _ _ => sorry -/
