lakefile.lean
@@ -4,8 +4,5 @@ open Lake DSL
 package «plfl» where
   -- add package configuration options here
 
-require mathlib from git
-  "https://github.com/leanprover-community/mathlib4.git"
-
 lean_lib «Plfl» where
   -- add library configuration options here
